main/hl/solutions/lean/LF/Typeclasses.lean
@@ -1712,4 +1712,4 @@ example {α : Type} (x : α) [BEq α] [LawfulBEq α] (xs : List α)
 
 end Reflection
 
--- Built on 2026-09-14 10:31 UTC
+-- Built on 2026-09-15 21:42 UTC
