main/lf/solutions/lean/LF/Basics.lean
@@ -2270,4 +2270,4 @@ theorem inspectBag_changeBag_comm_ticketed
 end Airport
 end NatPlayground
 
--- Built on 2026-09-14 10:30 UTC
+-- Built on 2026-09-15 21:40 UTC
