main/lf/student/lean/LF/Tactics.lean
@@ -1222,16 +1222,16 @@ theorem map_injective_of_injective {α β : Type}
     l₁ = l₂ := by
   sorry
 
---  ### Exercise (3 stars): unzip_zip (Advanced, Manually graded) ⭐⭐⭐
+--  ### Exercise (3 stars): unzip'_zip (Advanced, Manually graded) ⭐⭐⭐
 
 --  We proved in `zip_unzip'` that `zip`ping the result of `unzip'`
 --  recovers the original list. What about the other direction? Complete
---  and prove the following `unzip_zip`:
+--  and prove the following `unzip'_zip`:
 --
---      theorem unzip_zip {α β : Type}
+--      theorem unzip'_zip {α β : Type}
 --          {l₁ : List α} {l₂ : List β}
 --          /- add appropriate parameters and hypotheses here -/ :
---          unzip (zip l₁ l₂) = (l₁, l₂) := sorry
+--          unzip' (zip l₁ l₂) = (l₁, l₂) := sorry
 --
 --  Hint: Take a look at the definition of `zip` in Poly. Your definition
 --  will need to account for the behavior of `zip` in its base cases, which
@@ -1282,4 +1282,4 @@ theorem anyTrue_eq_anyTrue (α : Type) (test : α → Bool) (l : List α) :
     anyTrue test l = anyTrue' test l := by
   sorry
 
--- Built on 2026-09-14 10:29 UTC
+-- Built on 2026-09-15 21:40 UTC
