main/lf/terse/lean/LF/Poly.lean
@@ -687,4 +687,4 @@ def fold_plus : List Nat → Nat → Nat :=
 --  Output:
 --    fold_plus : List Nat → Nat → Nat
 
--- Built on 2026-09-14 10:30 UTC
+-- Built on 2026-09-15 21:41 UTC
