main/lf/terse/lean/LF/Postscript.lean
@@ -68,4 +68,4 @@ import SFLCompat
 --    develops formalized mathematics using Lean and
 --    Mathlib.
 
--- Built on 2026-09-14 10:30 UTC
+-- Built on 2026-09-15 21:41 UTC
